Prototype the RA for the model

src/verification/simpleapiserver.v
@@ -1,8 +1,9 @@
 From Perennial.algebra Require Export auth_map.
 From New.proof.github_com.goose_lang.goose.model.channel Require Export auth_set.
-Require Import New.proof.sync.
-From New.generatedproof.kubernetes_model Require Export simpleapiserver.
+Require Export New.proof.sync.
+
 From verification.kubernetes_model Require Export simpleapiserver_init.
+From verification Require Import prelude empty_ffi.
 Export simpleapiserver.simpleapiserver.
 
 Module KKey.
@@ -31,11 +32,16 @@ End KObject.
 Global Existing Instance KKey.eq_dec.
 Global Existing Instance KKey.countable.
 
-Section model.
-Context `{heapGS Σ, !ffi_semantics _ _}.
+Section proof.
+Context `{hG: !heapGS Σ} {go_ctx: GoContext}.
 Context `{!mapG Σ KKey.t interface.t}.
 Context `{!mapG Σ KKey.t KObject.t}.
+Context `{!mapG Σ KKey.t (gset KKey.t)}.
 Context `{!auth_setG Σ KKey.t}.
+
+Definition mk_pod_key (namespace name: go_string) : KKey.t :=
+  {| KKey.Kind' := "Pod"%go; KKey.Namespace' := namespace; KKey.Name' := name;|}.
+
 
 Definition pod_well_formed (pod: v1.Pod.t) (namespace name: go_string) : Prop :=
  True.
@@ -62,15 +68,85 @@ Definition state_rep (phys_state: gmap KKey.t interface.t) (abs_state: gmap KKey
     else False%I.
 
 
-Definition is_kubernetes_state_inner (l: loc) γ_state γ_fresh_keys: iProp Σ :=
-  ∃ (phys_state: gmap KKey.t interface.t) (abs_state: gmap KKey.t KObject.t) (s_fresh_keys: gset KKey.t),
-    "Hphys" ∷ l ↦$ phys_state ∗
-    "Habs" ∷ map_ctx γ_state 1 abs_state ∗
-    "Hrep" ∷ state_rep phys_state abs_state ∗
-    "Hfreshkeys" ∷ auth_set_auth γ_fresh_keys s_fresh_keys.
+Definition kubernetes_state_consistent (abs_state: gmap KKey.t KObject.t) (children: gmap KKey.t (gset KKey.t)) (fresh_keys: gset KKey.t): Prop := 
+  True.
 
 
-Definition is_kubernetes_state (l: loc) γ_state γ_fresh_keys : iProp Σ :=
-  ∃ mu_l, "#Hkinv" ∷ is_Mutex mu_l (is_kubernetes_state_inner l γ_state γ_fresh_keys).
+Definition is_kubernetes_state_inner γ_state γ_children γ_fresh_keys: iProp Σ :=
+  ∃ (l: loc) (phys_state: gmap KKey.t interface.t) (abs_state: gmap KKey.t KObject.t) (children: gmap KKey.t (gset KKey.t)) (fresh_keys: gset KKey.t),
+    "state_m_addr" ∷ (global_addr simpleapiserver.state) ↦s[ simpleapiserver.State :: "m" ] l ∗
+    "own_phys" ∷ l ↦$ phys_state ∗
+    "own_abs" ∷ map_ctx γ_state 1 abs_state ∗
+    "phys_abs_rep" ∷ state_rep phys_state abs_state ∗
+    "own_children" ∷ map_ctx γ_children 1 children ∗
+    "own_fresh_keys" ∷ auth_set_auth γ_fresh_keys fresh_keys ∗
+    "consistent" ∷ ⌜ kubernetes_state_consistent abs_state children fresh_keys ⌝ .
 
-End model.
+
+Definition is_kubernetes_state γ_state γ_children γ_fresh_keys : iProp Σ :=
+  is_Mutex (global_addr simpleapiserver.stateMu) (is_kubernetes_state_inner γ_state γ_children γ_fresh_keys).
+
+Lemma wp_objGet (key: KKey.t) γ_state γ_children γ_fresh_keys:
+  {{{ is_pkg_init simpleapiserver ∗
+      "#inv" ∷ is_kubernetes_state γ_state γ_children γ_fresh_keys
+  }}}
+    @! simpleapiserver.objGet #key
+  {{{ (obj: interface.t) (exists': bool), RET (#obj, #exists');
+    True
+  }}}.
+Proof.
+  wp_start as "H". iNamed "H".
+  wp_apply wp_with_defer. simpl subst.
+  iIntros (defer) "defer". wp_auto. iRename "key" into "kep_ptr".
+  wp_apply wp_globals_get.
+  wp_apply wp_Mutex__Lock.
+  { done. }
+  iIntros "[own_Mutex H]". iNamed "H". wp_auto.
+  wp_apply wp_globals_get. wp_apply wp_globals_get.
+  wp_apply (wp_map_get with "[$own_phys]").
+  iIntros "own_phys". wp_auto.
+  wp_apply (wp_Mutex__Unlock _ (is_kubernetes_state_inner γ_state γ_children γ_fresh_keys)
+    with "[$own_Mutex state_m_addr own_phys own_abs phys_abs_rep own_children own_fresh_keys consistent]").
+  { iFrame. done. }
+  iApply ("HΦ" $! (default interface.nil (phys_state !! key))
+                 (bool_decide (is_Some (phys_state !! key)))).
+  done.
+Qed.
+
+
+Lemma wp_PodGet (namespace name: go_string) γ_state γ_children γ_fresh_keys:
+  {{{ is_pkg_init simpleapiserver ∗
+      is_kubernetes_state γ_state γ_children γ_fresh_keys
+  }}}
+    @! simpleapiserver.PodGet #namespace #name
+  {{{ (l: loc) (err: error.t) dq2 (pod: v1.Pod.t), RET (#l, #err);
+    if decide (err = interface.nil) then
+      l ↦{dq2} pod
+    else
+      True
+  }}}.
+  wp_start as "H". iNamed "H".
+Admitted.
+
+
+Lemma wp_PodGet_with_ptsto_mut_state (namespace name: go_string) γ_state γ_children γ_fresh_keys dq pod:
+  {{{ is_pkg_init simpleapiserver ∗
+      is_kubernetes_state γ_state γ_children γ_fresh_keys ∗
+      ptsto_mut γ_state (mk_pod_key namespace name) dq (KObject.Pod pod)
+  }}}
+    @! simpleapiserver.PodGet #namespace #name
+  {{{ (l: loc) (err: error.t) dq2, RET (#l, #err);
+    ⌜ err = interface.nil ⌝ ∗
+    l ↦{dq2} pod ∗
+    ptsto_mut γ_state (mk_pod_key namespace name) dq (KObject.Pod pod)
+  }}}.
+Admitted.
+
+
+(* Lemma wp_PodList_with_ptsto_mut_children (namespace: go_string) (l: loc) γ_state γ_fresh_keys dq pods:
+  {{{ is_pkg_init simpleapiserver ∗
+      is_kubernetes_state l γ_state γ_fresh_keys ∗
+
+  }}} *)
+
+End proof.
